Make sure quickcode definitions use va_ prefix

tools/Vale/src/emit_common_lemmas.fs
@@ -662,7 +662,7 @@ let build_lemma (env:env) (benv:build_env) (b1:id) (stmts:stmt list) (bstmts:stm
       ]
     )
     else if benv.is_quick then (
-      let range = evar (Id "range1") in
+      let range = evar (Reserved "range1") in
       let msg = EString ("***** MODIFIES CLAUSE NOT MET AT " + string_of_loc loc + " *****") in
       let eFrameX = vaApp "state_match" [evar sM; eFrameExp] in
       let eFrameL = eapply (Id "label") [range; msg; eFrameX] in
