fstar/code/arch/x64/X64.Vale.QuickCode.fst
@@ -15,6 +15,7 @@ type mod_t =
 | Mod_flags: mod_t
 | Mod_mem: mod_t
 unfold let mods_t = list mod_t
+unfold let va_mods_t = mods_t
 
 [@va_qattr] unfold let va_Mod_None = Mod_None
 [@va_qattr] unfold let va_Mod_ok = Mod_ok
@@ -53,7 +54,7 @@ let rec update_state_mods (mods:mods_t) (sM sK:state) : state =
 unfold let update_state_mods_norm (mods:mods_t) (sM sK:state) : state =
   norm [iota; zeta; delta_attr [`%qmodattr]; delta_only [`%update_state_mods; `%update_state_mod]] (update_state_mods mods sM sK)
 
-let lemma_norm_mods (mods:mods_t) (sM sK:state) : Lemma
+let va_lemma_norm_mods (mods:mods_t) (sM sK:state) : Lemma
   (ensures update_state_mods mods sM sK == update_state_mods_norm mods sM sK)
   = ()
 
@@ -76,14 +77,15 @@ let va_mod_reg_opr64 (o:operand) : mod_t =
 let quickProc_wp (a:Type0) : Type u#1 = (s0:state) -> (wp_continue:state -> a -> Type0) -> Type0
 
 let t_require (s0:state) = state_inv s0
+unfold let va_t_require = t_require
 
-let t_ensure (#a:Type0) (c:va_code) (mods:mods_t) (s0:state) (k:(state -> a -> Type0)) =
+let va_t_ensure (#a:Type0) (c:va_code) (mods:mods_t) (s0:state) (k:(state -> a -> Type0)) =
   fun (sM, f0, g) -> eval_code c s0 f0 sM /\ update_state_mods mods sM s0 == sM /\ state_inv sM /\ k sM g
 
 let t_proof (#a:Type0) (c:va_code) (mods:mods_t) (wp:quickProc_wp a) : Type =
   s0:state -> k:(state -> a -> Type0) -> Ghost (state & va_fuel & a)
     (requires t_require s0 /\ wp s0 k)
-    (ensures t_ensure c mods s0 k)
+    (ensures va_t_ensure c mods s0 k)
 
 // Code that returns a ghost value of type a
 [@va_qattr]
@@ -95,6 +97,8 @@ noeq type quickCode (a:Type0) : va_code -> Type =
     proof:t_proof c mods wp ->
     quickCode a c
 
+[@va_qattr]
 unfold let va_quickCode = quickCode
+
 [@va_qattr]
 unfold let va_QProc = QProc
