fstar/code/arch/x64/X64.Vale.QuickCodes.fsti
@@ -52,12 +52,12 @@ noeq type quickCodes (a:Type0) : codes -> Type =
 | QSeq: #b:Type -> #c:code -> #cs:codes -> r:range -> msg:string ->
     quickCode b c -> quickCodes a cs -> quickCodes a (c::cs)
 | QBind: #b:Type -> #c:code -> #cs:codes -> r:range -> msg:string ->
-    quickCode b c -> (state -> b -> GTot (quickCodes a cs)) -> quickCodes a (c::cs)
-| QGetState: #cs:codes -> (state -> GTot (quickCodes a cs)) -> quickCodes a ((Block [])::cs)
+    quickCode b c -> (va_state -> b -> GTot (quickCodes a cs)) -> quickCodes a (c::cs)
+| QGetState: #cs:codes -> (va_state -> GTot (quickCodes a cs)) -> quickCodes a ((Block [])::cs)
 | QPURE: #cs:codes -> r:range -> msg:string -> pre:((unit -> GTot Type0) -> GTot Type0) ->
     (unit -> PURE unit pre) -> quickCodes a cs -> quickCodes a cs
 //| QBindPURE: #cs:codes -> b:Type -> r:range -> msg:string -> pre:((b -> GTot Type0) -> GTot Type0) ->
-//    (unit -> PURE b pre) -> (state -> b -> GTot (quickCodes a cs)) -> quickCodes a ((Block [])::cs)
+//    (unit -> PURE b pre) -> (va_state -> b -> GTot (quickCodes a cs)) -> quickCodes a ((Block [])::cs)
 | QLemma: #cs:codes -> r:range -> msg:string -> pre:Type0 -> post:(squash pre -> Type0) ->
     (unit -> Lemma (requires pre) (ensures post ())) -> quickCodes a cs -> quickCodes a cs
 | QGhost: #cs:codes -> b:Type -> r:range -> msg:string -> pre:Type0 -> post:(b -> Type0) ->
@@ -65,40 +65,45 @@ noeq type quickCodes (a:Type0) : codes -> Type =
 | QAssertBy: #cs:codes -> r:range -> msg:string -> p:Type0 ->
     quickCodes unit [] -> quickCodes a cs -> quickCodes a cs
 
+[@va_qattr] unfold let va_QBind (#a:Type0) (#b:Type) (#c:code) (#cs:codes) (r:range) (msg:string) (qc:quickCode b c) (qcs:va_state -> b -> GTot (quickCodes a cs)) : quickCodes a (c::cs) = QBind r msg qc qcs
+[@va_qattr] unfold let va_QEmpty (#a:Type0) (v:a) : quickCodes a [] = QEmpty v
+[@va_qattr] unfold let va_QLemma (#a:Type0) (#cs:codes) (r:range) (msg:string) (pre:Type0) (post:(squash pre -> Type0)) (l:unit -> Lemma (requires pre) (ensures post ())) (qcs:quickCodes a cs) : quickCodes a cs = QLemma r msg pre post l qcs
+[@va_qattr] unfold let va_QSeq (#a:Type0) (#b:Type) (#c:code) (#cs:codes) (r:range) (msg:string) (qc:quickCode b c) (qcs:quickCodes a cs) : quickCodes a (c::cs) = QSeq r msg qc qcs
+
 [@va_qattr]
-let qPURE
+let va_qPURE
     (#cs:codes) (#pre:(unit -> GTot Type0) -> GTot Type0) (#a:Type0) (r:range) (msg:string)
     ($l:unit -> PURE unit pre) (qcs:quickCodes a cs)
   : quickCodes a cs =
   QPURE r msg pre l qcs
 
-(* REVIEW: this might be useful, but inference of pre doesn't work as well as for qPURE
+(* REVIEW: this might be useful, but inference of pre doesn't work as well as for va_qPURE
   (need to provide pre explicitly; as a result, no need to put $ on l)
 [@va_qattr]
-let qBindPURE
+let va_qBindPURE
     (#a #b:Type0) (#cs:codes) (pre:(b -> GTot Type0) -> GTot Type0) (r:range) (msg:string)
-    (l:unit -> PURE b pre) (qcs:state -> b -> GTot (quickCodes a cs))
+    (l:unit -> PURE b pre) (qcs:va_state -> b -> GTot (quickCodes a cs))
   : quickCodes a ((Block [])::cs) =
   QBindPURE b r msg pre l qcs
 *)
 
 [@va_qattr]
-let wp_proc (#a:Type0) (c:code) (qc:quickCode a c) (s0:state) (k:state -> a -> Type0) : Type0 =
+let wp_proc (#a:Type0) (c:code) (qc:quickCode a c) (s0:va_state) (k:va_state -> a -> Type0) : Type0 =
   match qc with
   | QProc _ _ wp _ -> wp s0 k
 
-let wp_Seq_t (a:Type0) = state -> a -> Type0
-let wp_Bind_t (a:Type0) = state -> a -> Type0
-let k_AssertBy (p:Type0) (_:state) () = p
+let wp_Seq_t (a:Type0) = va_state -> a -> Type0
+let wp_Bind_t (a:Type0) = va_state -> a -> Type0
+let k_AssertBy (p:Type0) (_:va_state) () = p
 
 [@va_qattr]
-let range1 = mk_range "" 0 0 0 0
+let va_range1 = mk_range "" 0 0 0 0
 
 val empty_list_is_small (#a:Type) (x:list a) : Lemma
   ([] #a == x \/ [] #a << x)
 
 [@va_qattr]
-let rec wp (#a:Type0) (cs:codes) (qcs:quickCodes a cs) (mods:mods_t) (k:state -> a -> Type0) (s0:state) :
+let rec wp (#a:Type0) (cs:codes) (qcs:quickCodes a cs) (mods:mods_t) (k:va_state -> a -> Type0) (s0:va_state) :
   Tot Type0 (decreases %[cs; 0; qcs])
   =
   match qcs with
@@ -139,17 +144,17 @@ let rec wp (#a:Type0) (cs:codes) (qcs:quickCodes a cs) (mods:mods_t) (k:state ->
       wp [] qcsBy mods (k_AssertBy p) s0 /\ (p ==> wp cs qcs mods k s0)
 
 // Hoist lambdas out of main definition to avoid issues with function equality
-and wp_Seq (#a:Type0) (#b:Type0) (cs:codes) (qcs:quickCodes b cs) (mods:mods_t) (k:state -> b -> Type0) :
+and wp_Seq (#a:Type0) (#b:Type0) (cs:codes) (qcs:quickCodes b cs) (mods:mods_t) (k:va_state -> b -> Type0) :
   Tot (wp_Seq_t a) (decreases %[cs; 1; qcs])
   =
   let f s0 _ = wp cs qcs mods k s0 in f
-and wp_Bind (#a:Type0) (#b:Type0) (cs:codes) (qcs:state -> a -> GTot (quickCodes b cs)) (mods:mods_t) (k:state -> b -> Type0) :
+and wp_Bind (#a:Type0) (#b:Type0) (cs:codes) (qcs:va_state -> a -> GTot (quickCodes b cs)) (mods:mods_t) (k:va_state -> b -> Type0) :
   Tot (wp_Bind_t a) (decreases %[cs; 1; qcs])
   =
   let f s0 g = wp cs (qcs s0 g) mods k s0 in f
 
-val wp_sound (#a:Type0) (cs:codes) (qcs:quickCodes a cs) (mods:mods_t) (k:state -> a -> Type0) (s0:state)
-  : Ghost (state & va_fuel & a)
+val wp_sound (#a:Type0) (cs:codes) (qcs:quickCodes a cs) (mods:mods_t) (k:va_state -> a -> Type0) (s0:va_state)
+  : Ghost (va_state & va_fuel & a)
   (requires t_require s0 /\ wp cs qcs mods k s0)
   (ensures fun (sN, fN, gN) ->
     eval (Block cs) s0 fN sN /\ update_state_mods mods sN s0 == sN /\ state_inv sN /\ k sN gN
@@ -160,37 +165,37 @@ val wp_sound (#a:Type0) (cs:codes) (qcs:quickCodes a cs) (mods:mods_t) (k:state 
 unfold let block = va_Block
 
 [@va_qattr]
-let wp_block (#a:Type) (#cs:codes) (qcs:state -> GTot (quickCodes a cs)) (mods:mods_t) (s0:state) (k:state -> a -> Type0) : Type0 =
+let wp_block (#a:Type) (#cs:codes) (qcs:va_state -> GTot (quickCodes a cs)) (mods:mods_t) (s0:va_state) (k:va_state -> a -> Type0) : Type0 =
   wp cs (qcs s0) mods k s0
 
-val qblock_proof (#a:Type) (#cs:codes) (qcs:state -> GTot (quickCodes a cs)) (mods:mods_t) (s0:state) (k:state -> a -> Type0)
-  : Ghost (state & va_fuel & a)
+val qblock_proof (#a:Type) (#cs:codes) (qcs:va_state -> GTot (quickCodes a cs)) (mods:mods_t) (s0:va_state) (k:va_state -> a -> Type0)
+  : Ghost (va_state & va_fuel & a)
   (requires t_require s0 /\ wp_block qcs mods s0 k)
   (ensures fun (sM, f0, g) ->
     eval_code (block cs) s0 f0 sM /\ update_state_mods mods sM s0 == sM /\ state_inv sM /\ k sM g
   )
 
 [@"opaque_to_smt" va_qattr]
-let qblock (#a:Type) (#cs:codes) (mods:mods_t) (qcs:state -> GTot (quickCodes a cs)) : quickCode a (block cs) =
+let qblock (#a:Type) (#cs:codes) (mods:mods_t) (qcs:va_state -> GTot (quickCodes a cs)) : quickCode a (block cs) =
   QProc (block cs) mods (wp_block qcs mods) (qblock_proof qcs mods)
 
 ///// If, InlineIf
 
 [@va_qattr]
-let wp_InlineIf (#a:Type) (#c1:code) (#c2:code) (b:bool) (qc1:quickCode a c1) (qc2:quickCode a c2) (mods:mods_t) (s0:state) (k:state -> a -> Type0) : Type0 =
+let wp_InlineIf (#a:Type) (#c1:code) (#c2:code) (b:bool) (qc1:quickCode a c1) (qc2:quickCode a c2) (mods:mods_t) (s0:va_state) (k:va_state -> a -> Type0) : Type0 =
   // REVIEW: this duplicates k
   (    b ==> mods_contains mods qc1.mods /\ QProc?.wp qc1 s0 k) /\
   (not b ==> mods_contains mods qc2.mods /\ QProc?.wp qc2 s0 k)
 
-val qInlineIf_proof (#a:Type) (#c1:code) (#c2:code) (b:bool) (qc1:quickCode a c1) (qc2:quickCode a c2) (mods:mods_t) (s0:state) (k:state -> a -> Type0)
-  : Ghost (state & va_fuel & a)
+val qInlineIf_proof (#a:Type) (#c1:code) (#c2:code) (b:bool) (qc1:quickCode a c1) (qc2:quickCode a c2) (mods:mods_t) (s0:va_state) (k:va_state -> a -> Type0)
+  : Ghost (va_state & va_fuel & a)
   (requires t_require s0 /\ wp_InlineIf b qc1 qc2 mods s0 k)
   (ensures fun (sM, f0, g) ->
     eval_code (if_code b c1 c2) s0 f0 sM /\ update_state_mods mods sM s0 == sM /\ state_inv sM /\ k sM g
   )
 
 [@"opaque_to_smt" va_qattr]
-let qInlineIf (#a:Type) (#c1:code) (#c2:code) (mods:mods_t) (b:bool) (qc1:quickCode a c1) (qc2:quickCode a c2) : quickCode a (if_code b c1 c2) =
+let va_qInlineIf (#a:Type) (#c1:code) (#c2:code) (mods:mods_t) (b:bool) (qc1:quickCode a c1) (qc2:quickCode a c2) : quickCode a (if_code b c1 c2) =
   QProc (if_code b c1 c2) mods (wp_InlineIf b qc1 qc2 mods) (qInlineIf_proof b qc1 qc2 mods)
 
 type cmp =
@@ -212,7 +217,7 @@ let cmp_to_ocmp (c:cmp) : ocmp =
   | Cmp_gt o1 o2 -> va_cmp_gt o1 o2
 
 [@va_qattr]
-let valid_cmp (c:cmp) (s:state) : Type0 =
+let valid_cmp (c:cmp) (s:va_state) : Type0 =
   match c with
   | Cmp_eq o1 o2 -> valid_operand o1 s /\ valid_operand o2 s
   | Cmp_ne o1 o2 -> valid_operand o1 s /\ valid_operand o2 s
@@ -222,7 +227,7 @@ let valid_cmp (c:cmp) (s:state) : Type0 =
   | Cmp_gt o1 o2 -> valid_operand o1 s /\ valid_operand o2 s
 
 [@va_qattr]
-let eval_cmp (s:state) (c:cmp) : GTot bool =
+let eval_cmp (s:va_state) (c:cmp) : GTot bool =
   match c with
   | Cmp_eq o1 o2 -> va_eval_opr64 s o1 =  va_eval_opr64 s o2
   | Cmp_ne o1 o2 -> va_eval_opr64 s o1 <> va_eval_opr64 s o2
@@ -232,36 +237,36 @@ let eval_cmp (s:state) (c:cmp) : GTot bool =
   | Cmp_gt o1 o2 -> va_eval_opr64 s o1 >  va_eval_opr64 s o2
 
 [@va_qattr]
-let wp_If (#a:Type) (#c1:code) (#c2:code) (b:cmp) (qc1:quickCode a c1) (qc2:quickCode a c2) (mods:mods_t) (s0:state) (k:state -> a -> Type0) : Type0 =
+let wp_If (#a:Type) (#c1:code) (#c2:code) (b:cmp) (qc1:quickCode a c1) (qc2:quickCode a c2) (mods:mods_t) (s0:va_state) (k:va_state -> a -> Type0) : Type0 =
   // REVIEW: this duplicates k
   valid_cmp b s0 /\
   (     eval_cmp s0 b  ==> mods_contains mods qc1.mods /\ QProc?.wp qc1 s0 k) /\
   (not (eval_cmp s0 b) ==> mods_contains mods qc2.mods /\ QProc?.wp qc2 s0 k)
 
-val qIf_proof (#a:Type) (#c1:code) (#c2:code) (b:cmp) (qc1:quickCode a c1) (qc2:quickCode a c2) (mods:mods_t) (s0:state) (k:state -> a -> Type0)
-  : Ghost (state & va_fuel & a)
+val qIf_proof (#a:Type) (#c1:code) (#c2:code) (b:cmp) (qc1:quickCode a c1) (qc2:quickCode a c2) (mods:mods_t) (s0:va_state) (k:va_state -> a -> Type0)
+  : Ghost (va_state & va_fuel & a)
   (requires t_require s0 /\ wp_If b qc1 qc2 mods s0 k)
   (ensures fun (sM, f0, g) ->
     eval_code (IfElse (cmp_to_ocmp b) c1 c2) s0 f0 sM /\ update_state_mods mods sM s0 == sM /\ state_inv sM /\ k sM g
   )
 
 [@"opaque_to_smt" va_qattr]
-let qIf (#a:Type) (#c1:code) (#c2:code) (mods:mods_t) (b:cmp) (qc1:quickCode a c1) (qc2:quickCode a c2) : quickCode a (IfElse (cmp_to_ocmp b) c1 c2) =
+let va_qIf (#a:Type) (#c1:code) (#c2:code) (mods:mods_t) (b:cmp) (qc1:quickCode a c1) (qc2:quickCode a c2) : quickCode a (IfElse (cmp_to_ocmp b) c1 c2) =
   QProc (IfElse (cmp_to_ocmp b) c1 c2) mods (wp_If b qc1 qc2 mods) (qIf_proof b qc1 qc2 mods)
 
 ///// While
 
 [@va_qattr]
 let wp_While_inv
-    (#a #d:Type) (#c:code) (qc:a -> quickCode a c) (mods:mods_t) (inv:state -> a -> Type0)
-    (dec:state -> a -> d) (s1:state) (g1:a) (s2:state) (g2:a)
+    (#a #d:Type) (#c:code) (qc:a -> quickCode a c) (mods:mods_t) (inv:va_state -> a -> Type0)
+    (dec:va_state -> a -> d) (s1:va_state) (g1:a) (s2:va_state) (g2:a)
     : Type0 =
   s2.ok /\ inv s2 g2 /\ mods_contains mods (qc g2).mods /\ dec s2 g2 << dec s1 g1
 
 [@va_qattr]
 let wp_While_body
-    (#a #d:Type) (#c:code) (b:cmp) (qc:a -> quickCode a c) (mods:mods_t) (inv:state -> a -> Type0)
-    (dec:state -> a -> d) (g1:a) (s1:state) (k:state -> a -> Type0)
+    (#a #d:Type) (#c:code) (b:cmp) (qc:a -> quickCode a c) (mods:mods_t) (inv:va_state -> a -> Type0)
+    (dec:va_state -> a -> d) (g1:a) (s1:va_state) (k:va_state -> a -> Type0)
     : Type0 =
   valid_cmp b s1 /\
   (     eval_cmp s1 b  ==> mods_contains mods (qc g1).mods /\ QProc?.wp (qc g1) s1 (wp_While_inv qc mods inv dec s1 g1)) /\
@@ -269,26 +274,26 @@ let wp_While_body
 
 [@va_qattr]
 let wp_While
-    (#a #d:Type) (#c:code) (b:cmp) (qc:a -> quickCode a c) (mods:mods_t) (inv:state -> a -> Type0)
-    (dec:state -> a -> d) (g0:a) (s0:state) (k:state -> a -> Type0)
+    (#a #d:Type) (#c:code) (b:cmp) (qc:a -> quickCode a c) (mods:mods_t) (inv:va_state -> a -> Type0)
+    (dec:va_state -> a -> d) (g0:a) (s0:va_state) (k:va_state -> a -> Type0)
     : Type0 =
   inv s0 g0 /\ mods_contains mods (qc g0).mods /\
-  // REVIEW: we could get a better WP with forall (...state components...) instead of forall (s1:state)
-  (forall (s1:state) (g1:a). inv s1 g1 ==> wp_While_body b qc mods inv dec g1 s1 k)
+  // REVIEW: we could get a better WP with forall (...va_state components...) instead of forall (s1:va_state)
+  (forall (s1:va_state) (g1:a). inv s1 g1 ==> wp_While_body b qc mods inv dec g1 s1 k)
 
 val qWhile_proof
-    (#a #d:Type) (#c:code) (b:cmp) (qc:a -> quickCode a c) (mods:mods_t) (inv:state -> a -> Type0)
-    (dec:state -> a -> d) (g0:a) (s0:state) (k:state -> a -> Type0)
-  : Ghost (state & va_fuel & a)
+    (#a #d:Type) (#c:code) (b:cmp) (qc:a -> quickCode a c) (mods:mods_t) (inv:va_state -> a -> Type0)
+    (dec:va_state -> a -> d) (g0:a) (s0:va_state) (k:va_state -> a -> Type0)
+  : Ghost (va_state & va_fuel & a)
   (requires t_require s0 /\ wp_While b qc mods inv dec g0 s0 k)
   (ensures fun (sM, f0, g) ->
     eval_code (While (cmp_to_ocmp b) c) s0 f0 sM /\ update_state_mods mods sM s0 == sM /\ state_inv sM /\ k sM g
   )
 
 [@"opaque_to_smt" va_qattr]
-let qWhile
-    (#a #d:Type) (#c:code) (mods:mods_t) (b:cmp) (qc:a -> quickCode a c) (inv:state -> a -> Type0)
-    (dec:state -> a -> d) (g0:a)
+let va_qWhile
+    (#a #d:Type) (#c:code) (mods:mods_t) (b:cmp) (qc:a -> quickCode a c) (inv:va_state -> a -> Type0)
+    (dec:va_state -> a -> d) (g0:a)
   : quickCode a (While (cmp_to_ocmp b) c) =
   QProc (While (cmp_to_ocmp b) c) mods (wp_While b qc mods inv dec g0)
     (qWhile_proof b qc mods inv dec g0)
@@ -299,41 +304,41 @@ let tAssertLemma (p:Type0) = unit -> Lemma (requires p) (ensures p)
 val qAssertLemma (p:Type0) : tAssertLemma p
 
 [@va_qattr]
-let qAssert (#a:Type) (#cs:codes) (r:range) (msg:string) (e:Type0) (qcs:quickCodes a cs) : quickCodes a cs =
+let va_qAssert (#a:Type) (#cs:codes) (r:range) (msg:string) (e:Type0) (qcs:quickCodes a cs) : quickCodes a cs =
   QLemma r msg e (fun () -> e) (qAssertLemma e) qcs
 
 let tAssumeLemma (p:Type0) = unit -> Lemma (requires True) (ensures p)
 val qAssumeLemma (p:Type0) : tAssumeLemma p
 
 [@va_qattr]
-let qAssume (#a:Type) (#cs:codes) (r:range) (msg:string) (e:Type0) (qcs:quickCodes a cs) : quickCodes a cs =
+let va_qAssume (#a:Type) (#cs:codes) (r:range) (msg:string) (e:Type0) (qcs:quickCodes a cs) : quickCodes a cs =
   QLemma r msg True (fun () -> e) (qAssumeLemma e) qcs
 
 let tAssertSquashLemma (p:Type0) = unit -> Ghost (squash p) (requires p) (ensures fun () -> p)
 val qAssertSquashLemma (p:Type0) : tAssertSquashLemma p
 
 [@va_qattr]
-let qAssertSquash
+let va_qAssertSquash
     (#a:Type) (#cs:codes) (r:range) (msg:string) (e:Type0) (qcs:squash e -> GTot (quickCodes a cs))
   : quickCodes a ((Block [])::cs) =
   QGhost (squash e) r msg e (fun () -> e) (qAssertSquashLemma e) qcs
 
-//let tAssertByLemma (#a:Type) (p:Type0) (qcs:quickCodes a []) (mods:mods_t) (s0:state) =
+//let tAssertByLemma (#a:Type) (p:Type0) (qcs:quickCodes a []) (mods:mods_t) (s0:va_state) =
 //  unit -> Lemma (requires t_require s0 /\ wp [] qcs mods (fun _ _ -> p) s0) (ensures p)
-//val qAssertByLemma (#a:Type) (p:Type0) (qcs:quickCodes a []) (mods:mods_t) (s0:state) : tAssertByLemma p qcs mods s0
+//val qAssertByLemma (#a:Type) (p:Type0) (qcs:quickCodes a []) (mods:mods_t) (s0:va_state) : tAssertByLemma p qcs mods s0
 //
 //[@va_qattr]
-//let qAssertBy (#a:Type) (#cs:codes) (mods:mods_t) (r:range) (msg:string) (p:Type0) (qcsBy:quickCodes unit []) (s0:state) (qcsTail:quickCodes a cs) : quickCodes a cs =
+//let va_qAssertBy (#a:Type) (#cs:codes) (mods:mods_t) (r:range) (msg:string) (p:Type0) (qcsBy:quickCodes unit []) (s0:va_state) (qcsTail:quickCodes a cs) : quickCodes a cs =
 //  QLemma r msg (t_require s0 /\ wp [] qcsBy mods (fun _ _ -> p) s0) (fun () -> p) (qAssertByLemma p qcsBy mods s0) qcsTail
 
 [@va_qattr]
-let qAssertBy (#a:Type) (#cs:codes) (r:range) (msg:string) (p:Type0) (qcsBy:quickCodes unit []) (qcsTail:quickCodes a cs) : quickCodes a cs =
+let va_qAssertBy (#a:Type) (#cs:codes) (r:range) (msg:string) (p:Type0) (qcsBy:quickCodes unit []) (qcsTail:quickCodes a cs) : quickCodes a cs =
   QAssertBy r msg p qcsBy qcsTail
 
 ///// Code
 
-val wp_sound_code (#a:Type0) (c:code) (qc:quickCode a c) (k:state -> a -> Type0) (s0:state) :
-  Ghost (state & fuel & a)
+val wp_sound_code (#a:Type0) (c:code) (qc:quickCode a c) (k:va_state -> a -> Type0) (s0:va_state) :
+  Ghost (va_state & fuel & a)
   (requires t_require s0 /\ QProc?.wp qc s0 k)
   (ensures fun (sN, fN, gN) -> eval_code c s0 fN sN /\ update_state_mods qc.mods sN s0 == sN /\ state_inv sN /\ k sN gN)
 
@@ -362,7 +367,7 @@ let all_xmms_match (r0:Xmms.t) (r1:Xmms.t) : Type0
   xmms_match xmms r0 r1
 
 [@va_qattr]
-let va_state_match (s0:state) (s1:state) : Pure Type0
+let va_state_match (s0:va_state) (s1:va_state) : Pure Type0
   (requires True)
   (ensures fun b -> b ==> state_eq s0 s1)
   =
@@ -375,12 +380,12 @@ let va_state_match (s0:state) (s1:state) : Pure Type0
   s0.mem == s1.mem
 
 [@va_qattr]
-unfold let wp_sound_code_pre (#a:Type0) (#c:code) (qc:quickCode a c) (s0:state) (k:(s0':state{s0 == s0'}) -> state -> a -> Type0) : Type0 =
+unfold let wp_sound_code_pre (#a:Type0) (#c:code) (qc:quickCode a c) (s0:va_state) (k:(s0':va_state{s0 == s0'}) -> va_state -> a -> Type0) : Type0 =
   forall (ok:bool) (regs:Regs.t) (xmms:Xmms.t) (flags:nat64) (mem:memory).
     let s0' = {ok = ok; regs = regs; xmms = xmms; flags = flags; mem = mem} in
     s0 == s0' ==> QProc?.wp qc s0' (k s0')
 
-unfold let wp_sound_code_post (#a:Type0) (#c:code) (qc:quickCode a c) (s0:state) (k:(s0':state{s0 == s0'}) -> state -> a -> Type0) ((sN:state), (fN:fuel), (gN:a)) : Type0 =
+unfold let wp_sound_code_post (#a:Type0) (#c:code) (qc:quickCode a c) (s0:va_state) (k:(s0':va_state{s0 == s0'}) -> va_state -> a -> Type0) ((sN:va_state), (fN:fuel), (gN:a)) : Type0 =
   eval c s0 fN sN /\
   update_state_mods qc.mods sN s0 == sN /\
   state_inv sN /\
@@ -403,8 +408,8 @@ unfold let normal_steps : list string =
 
 unfold let normal (x:Type0) : Type0 = norm [iota; zeta; simplify; primops; delta_attr [`%va_qattr]; delta_only normal_steps] x
 
-val wp_sound_code_norm (#a:Type0) (c:code) (qc:quickCode a c) (s0:state) (k:(s0':state{s0 == s0'}) -> state -> a -> Type0) :
-  Ghost (state & fuel & a)
+val va_wp_sound_code_norm (#a:Type0) (c:code) (qc:quickCode a c) (s0:va_state) (k:(s0':va_state{s0 == s0'}) -> va_state -> a -> Type0) :
+  Ghost (va_state & fuel & a)
     (t_require s0 /\ normal (wp_sound_code_pre qc s0 k))
     (wp_sound_code_post qc s0 k)
 
